UnitTest/BoundedBitblasting/BoundedBitblasting.lean
@@ -1,19 +1,47 @@
 import Veir.Meta.PBVDecide
 
+/-- Commutativity of addition -/
 example (w : Nat) (x y : BitVec w) (hw : w ≤ 4) :
   x + y = y + x := by
   pbv_decide 4
   · bv_decide
   · grind
 
+/-- Commutativity of addition for three variables -/
 example (w : Nat) (x y z : BitVec w) (hw : w ≤ 4) :
   x + y + z = y + x + z := by
   pbv_decide 4
   · bv_decide
   · grind
 
-example (w : Nat) (x : BitVec (w + 0)) (y : BitVec w) (hw : w ≤ 4) :
-  x + y = y + x := by
-  pbv_decide 4
+-- example (w : Nat) (x : BitVec (w + 0)) (y : BitVec w) (hw : w ≤ 4) :
+--   x + y = y + x := by
+--   pbv_decide 4
+--   · bv_decide
+--   · grind
+
+/-- Zero extending a zero extension-/
+example (p q r : Nat) (x : BitVec p)
+  (hr : r ≤ 8)
+  (hqr : q < r)
+  (hpq : p < q) :
+  (x.zeroExtend q).zeroExtend r = x.zeroExtend r
+  := by
+  pbv_decide 8
   · bv_decide
+  · grind
+  · grind
+  · grind
+
+/-- Sign extending a zero extensions -/
+example (p q r : Nat) (x : BitVec p)
+  (hr : r ≤ 8)
+  (hqr : q < r)
+  (hpq : p < q) :
+  (x.zeroExtend q).signExtend r = x.zeroExtend r
+  := by
+  pbv_decide 8
+  · bv_decide
+  · grind
+  · grind
   · grind
